Semantic/ModalCapybara/Syntax/SepCtx.lean
@@ -72,6 +72,53 @@ theorem SepCtx.rename_comp
   | cons K C m ih =>
     simp [SepCtx.rename, ih, CaptureSet.rename_comp]
 
+theorem SepCtx.Has.rename
+    {K : SepCtx s1} {f : Rename s1 s2}
+    (h : SepCtx.Has K C m) :
+    SepCtx.Has (K.rename f) (C.rename f) m := by
+  induction h with
+  | here => simp [SepCtx.rename]; exact .here
+  | there h ih => simp [SepCtx.rename]; exact .there ih
+
+theorem SepCtx.Has.rename_inv
+    {K : SepCtx s1} {f : Rename s1 s2}
+    (h : SepCtx.Has (K.rename f) C m) :
+    ∃ C0, C = C0.rename f ∧ SepCtx.Has K C0 m := by
+  induction K with
+  | empty =>
+    cases h
+  | cons K C0 m0 ih =>
+    simp [SepCtx.rename] at h
+    cases h with
+    | here =>
+      exact ⟨C0, rfl, .here⟩
+    | there h' =>
+      obtain ⟨C1, hC1, hh⟩ := ih h'
+      exact ⟨C1, hC1, .there hh⟩
+
+theorem SepCtx.HasTwoDistinct.rename
+    {K : SepCtx s1} {f : Rename s1 s2}
+    (h : SepCtx.HasTwoDistinct K C1 m1 C2 m2) :
+    SepCtx.HasTwoDistinct (K.rename f) (C1.rename f) m1 (C2.rename f) m2 := by
+  induction h with
+  | here_there hhas =>
+    simp [SepCtx.rename]
+    exact .here_there (hhas.rename)
+  | there h ih =>
+    simp [SepCtx.rename]
+    exact .there ih
+  | symm h ih =>
+    exact .symm ih
+
+theorem SepCtx.HasTwoDistinct.rename_inv
+    {K : SepCtx s1} {f : Rename s1 s2}
+    (h : SepCtx.HasTwoDistinct (K.rename f) C1 m1 C2 m2) :
+    ∃ D1 D2,
+      C1 = D1.rename f ∧
+      C2 = D2.rename f ∧
+      SepCtx.HasTwoDistinct K D1 m1 D2 m2 := by
+  sorry
+
 /-- A separation context is closed if it contains no heap pointers. -/
 inductive SepCtx.IsClosed : SepCtx s -> Prop where
 | empty : SepCtx.IsClosed .empty
